new code/countdown_compute.v
@@ -1,0 +1,150 @@
+Require Import Omega.
+Require Import prelims.
+Require Import countdown_repeater.
+
+
+(*
+=============================================================================
+**************** SECTION 4: COUNTDOWN COMPUTATIONS **************************
+=============================================================================
+*)
+
+(* This section contains the actual definition of countdown, as we previously
+   only work with its properties (i.e. what countdown should be, rather than
+   what it actually is.
+   I choose a different approach than my previous approach here, which is
+   actually simpler (very straighforward), but will require a longer proof of
+   correctness
+   What happened to the previous approach? I am trying to clean its code to
+   get rid of edge cases (e.g. check if (f n) is below 1 or not), not done yet
+   Also, this new approach is both simpler and faster. It takes o(n) time instead
+   of O(n) ! *)
+
+(* ****** 1.1. DEFINITION *************************************)
+
+
+(* Basically, repeats "f" "k" times or until we go below "a".
+   Output "min(k, min{l : repeat f l n <= a})" *)
+Fixpoint countdown_to_worker (a : nat) (f : nat -> nat) (n k : nat)
+: nat :=
+match k with
+| 0    => 0
+| S k' => match (n - a) with
+          | 0   => 0
+          | S _ => S (countdown_to_worker a f (f n) k') end
+end.
+
+(* Actual defintion. We give the worker a budget of "n" steps, which
+   guarantees it reach below "a" before terminating *)
+Definition countdown_to a f n := countdown_to_worker a f n n.
+
+
+(* ****** 1.2. THEOREMS ************************************* *)
+
+(* INITIAL VALUE THEOREM
+   Basically countdown returns 0 if "n" is already below "a" *)
+Theorem countdown_to_init : forall a f n k,
+(n <= a) -> (countdown_to_worker a f n k = 0).
+Proof.
+intros a f n k Hna.
+unfold countdown_to_worker.
+destruct k. { trivial. }
+replace (n - a) with 0 by omega.
+trivial.
+Qed.
+
+
+(* INTERMEDIATE STATE LEMMA
+   Similar to the general recursion formula for "countdown_to_recurse_rel" *)
+Theorem countdown_to_intermediate : forall a f n k i,
+contracting f
+-> S i <= k
+-> S a <= repeat f i n
+-> countdown_to_worker a f n k
+   = (S i) + countdown_to_worker a f (repeat f (S i) n) (k - (S i)).
+Proof.
+assert (forall a f n k, contracting f -> 1 <= k -> S a <= n
+        -> countdown_to_worker a f n k
+        = 1 + countdown_to_worker a f (f n) (k - 1)
+        ) as case_0.
+{ simpl. intros a f n k Hf Hk Ha.
+  destruct k. { omega. }
+  replace (S k - 1) with k by omega.
+  unfold countdown_to_worker.
+  replace (n-a) with (S(n - S a)) by omega.
+  trivial.
+}
+intros a f n k i Hf Hik Hai.
+induction i.
+{ simpl. apply case_0; trivial. }
+rewrite IHi.
+- simpl. remember (f (repeat f i n)) as m.
+  remember (k - S i) as l.
+  replace (k - S(S i)) with (l - 1) by omega.
+  rewrite case_0.
+  + omega.
+  + trivial.
+  + omega.
+  + simpl in Hai. rewrite Heqm. trivial.
+- omega.
+- apply (Nat.le_trans _ (repeat f (S i) n) _).
+  + trivial.
+  + apply Hf.
+Qed.
+
+(* COUNTDOWN VS REPEAT THEOREM
+   This is the correctness theorem for this countdown defintion 
+   It asserts that this countdown function obeys the conditions
+   set up for countdown in "countdown_repeater.v" *)
+Theorem countdown_to_repeat : forall a f,
+contracting f
+-> contract_strict_from (S a) f
+-> countdown_to_repeat_rel a f (countdown_to a f).
+Proof.
+intros a f Hf Haf n k.
+unfold countdown_to.
+split.
+- intro. rewrite not_lt. intro.
+  rewrite (countdown_to_intermediate a f n n k) in H.
+  + omega.
+  + apply Hf.
+  + apply (Nat.le_trans _ (S k + (repeat f (S k) n)) _).
+    * omega.
+    * apply (repeat_contract_strict a f n k). apply Hf. apply Haf. apply H0.
+  + apply H0.
+- intro. destruct k.
+  { simpl in H. rewrite (countdown_to_init a f n).
+    omega. apply H. }
+  remember (n - a) as m.
+  destruct m. { rewrite countdown_to_init; omega. }
+  destruct (repeat_contract_strict_threshold a f n).
+  + apply Hf.
+  + apply Haf.
+  + omega.
+  + destruct H0 as [Hx0 Hx1]. destruct Hx1 as [Hxl Hxr].
+    assert (countdown_to_worker a f n n = S x) as Hx.
+    { rewrite (countdown_to_intermediate a f n n x).
+      - rewrite countdown_to_init. omega. apply Hxl.
+      - apply Hf.
+      - apply Hx0.
+      - apply Hxr. }
+    rewrite Hx. apply not_le. intro.
+    apply (repeat_contract f n (S k) x) in H0.
+    omega. apply Hf.
+Qed.
+
+(* RECURSION FOR CONTRACTORS THEOREM *)
+Theorem countdown_to_contractor : forall a f n,
+contracting f
+-> contract_strict_from (S a) f
+-> S a <= n
+-> countdown_to a f n = S(countdown_to a f (f n)).
+Proof.
+intros a f n Hf Haf Han.
+assert (H0 := Hf).
+apply (countdown_to_repeat a f) in H0.
+- rewrite countdown_to_rel_recursion in H0.
+  destruct (H0 n) as [Hfn0 Hfn1].
+  tauto. apply Hf. apply Haf.
+- apply Haf.
+Qed.
