new code/countdown_repeater.v
@@ -1,0 +1,195 @@
+Require Import Omega.
+Require Import prelims.
+
+
+(*
+=============================================================================
+****************** SECTION 1: COUNTDOWN AND REPEATER ************************
+=============================================================================
+*)
+
+(* Countdown is non-trivial to define, our approach is to provide a sort of interface
+   for it by separating the core property and the actual definition. We provide the
+   relation "countdown_to_repeat_rel" to state the condition for "cf" to be the countdown
+   to "a" of "f". All facts about countdown can be proven just using this condition
+   without touching the real definition, which will be provided later *)
+
+(* ****** 1.1. COUNTDOWN ******************************* *)
+
+
+(* ****** 1.1.1. DEFINITIONS ********************)
+
+(* Basically says that "cf n" is the minimum number of times we need to
+   repeat "f" to get a result less than or equal to "a" *)
+Definition countdown_to_repeat_rel (a : nat) (f cf : nat -> nat) : Prop
+:= forall n k : nat, cf n <= k <-> repeat f k n <= a.
+
+
+(* Usual recursive property of countdown : "cf n = 1 + cf (f n)" *)
+Definition countdown_to_recurse_rel (a : nat) (f cf : nat -> nat) : Prop
+:= forall n, ((n <= a) -> cf n = 0) /\ ((S a <= n) -> cf n = S (cf (f n))).
+
+
+(* General formula derived from the recursive property above *)
+Lemma countdown_to_recurse_formula :
+forall a f cf n k, contracting f
+-> countdown_to_recurse_rel a f cf
+-> S a <= repeat f k n
+-> cf n = (S k) + cf (repeat f (S k) n).
+Proof.
+intros a f cf n k Hf Hfcf Han.
+induction k.
+{ simpl. simpl in Han. destruct (Hfcf n) as [_ Hfcfn].
+  apply Hfcfn. apply Han. }
+simpl in Han. rewrite IHk.
+- simpl. destruct (Hfcf (f (repeat f k n))) as [_ Hfcfn].
+  apply Hfcfn in Han. omega.
+- apply (Nat.le_trans _ (f (repeat f k n)) _).
+  + apply Han.
+  + apply Hf.
+Qed.
+
+
+(* Proof that the two above conditions are equivalent *)
+Theorem countdown_to_rel_recursion :
+forall a f cf, contracting f
+-> contract_strict_from (S a) f
+-> (countdown_to_repeat_rel a f cf <-> countdown_to_recurse_rel a f cf).
+Proof.
+intros a f cf Hf Haf.
+unfold countdown_to_repeat_rel.
+unfold countdown_to_recurse_rel.
+split.
+- intros Hfcf n. split.
+  + rewrite <- (Hfcf n 0). omega.
+  + intro Han. remember (cf (f n)) as k.
+    assert (cf n <= S k).
+    { rewrite Hfcf. rewrite repeat_S_comm.
+      rewrite <- Hfcf. omega. }
+    assert (~ cf n <= k).
+    { rewrite Hfcf. destruct k. { simpl. omega. }
+      rewrite repeat_S_comm. rewrite <- Hfcf.
+      omega. }
+    omega.
+- intros Hfcf n k. split.
+  + intro Hkn. rewrite not_lt. intro.
+    rewrite (countdown_to_recurse_formula a f cf n k) in Hkn.
+    * omega.
+    * apply Hf.
+    * unfold countdown_to_recurse_rel. apply Hfcf.
+    * apply H.
+  + remember (n - a) as m.
+    destruct m.
+    { intro. destruct (Hfcf n) as [Hfcfn _].
+      rewrite Hfcfn. omega. omega. }
+    assert (S a <= n) as Han by omega.
+    destruct (repeat_contract_strict_threshold a f n) as [x Hx].
+    * apply Hf.
+    * apply Haf.
+    * apply Han.
+    * intro. destruct Hx as [Hxn Hxna].
+      destruct Hxna as [Hxnal Hxnar].
+      assert (cf n = S x).
+      { rewrite (countdown_to_recurse_formula a f cf n x).
+        - destruct (Hfcf (repeat f (S x) n)) as [Hfcfxn _].
+          apply Hfcfxn in Hxnal. omega.
+        - apply Hf.
+        - unfold countdown_to_recurse_rel. apply Hfcf.
+        - apply Hxnar. }
+      rewrite H0. apply not_le. intro.
+      apply (repeat_contract f n k x) in Hf.
+      omega. apply H1.
+Qed.
+
+
+(* ****** 1.1.1. PROPERTIES ********************)
+
+
+(* Countdown preserves increasing-ness of contractions *)
+Theorem countdown_to_incr : forall a f cf,
+contracting f -> increasing f
+-> countdown_to_repeat_rel a f cf -> increasing cf.
+Proof.
+intros a f cf Hf0 Hf1 Hfcf n m Hnm.
+unfold countdown_to_repeat_rel in Hfcf.
+rewrite Hfcf.
+apply (Nat.le_trans _ (repeat f (cf m) m) _).
+- apply (repeat_incr (cf m) f) in Hf1. apply Hf1. apply Hnm.
+- rewrite <- Hfcf. trivial.
+Qed.
+
+
+(* Countdown preserves contracting-ness of contractions *)
+Theorem countdown_to_contract : forall a f cf,
+(1 <= a) -> contracting f
+-> contract_strict_from (S a) f
+-> countdown_to_repeat_rel a f cf
+-> contracting cf /\ contract_strict_from 1 cf.
+Proof.
+intros a f cf Ha Hf Haf Hfcf.
+split.
+- intro. rewrite (Hfcf n n).
+  rewrite not_lt. intro.
+  apply repeat_contract_strict in H.
+  + omega.
+  + apply Hf.
+  + apply Haf.
+- intros n Hn. destruct n. { omega. }
+  rewrite <- le_S_n_m. rewrite (Hfcf _ n).
+  destruct n. { trivial. }
+  remember (repeat f n (S (S n)) - a) as m.
+  destruct m.
+  { apply (Nat.le_trans _ (repeat f n (S (S n))) _).
+    apply Hf. omega. }
+  assert (S n + repeat f (S n) (S (S n)) <= (S n) + a).
+  { apply (Nat.le_trans _ (S (S n)) _).
+    apply (repeat_contract_strict a _ _).
+    - apply Hf.
+    - apply Haf.
+    - omega.
+    - omega. }
+  omega.
+Qed.
+
+(* Basically: "f" has a countdown to "a" if
+   it is a contraction that is strict from "a" *)
+Definition countdownable_to (a : nat) (f : nat -> nat) : Prop
+:= contracting f /\ contract_strict_from (S a) f.
+
+
+(* Just the combination of the two preservation theorems above *)
+Theorem countdown_countdownable : forall a f cf,
+(1 <= a) -> countdownable_to a f
+-> (countdown_to_repeat_rel a f cf)
+-> countdownable_to a cf.
+Proof.
+intros a f cf Ha Haf Hafcf.
+destruct Haf as [Haf0 Haf1].
+apply (countdown_to_contract a f cf) in Haf0.
+- destruct Haf0 as [Hcf0 Hcf1].
+  split.
+  + apply Hcf0.
+  + intros n Han. apply Hcf1. omega.
+- apply Ha.
+- apply Haf1.
+- apply Hafcf.
+Qed.
+
+
+(* ****** 1.2. REPEATER ******************************** *)
+
+(* Can be easily defined and computed, so we define it directly *)
+Fixpoint repeater_from (a : nat) (f : nat -> nat) (n : nat) : nat
+:= match n with
+   | 0 => a
+   | S n' => f (repeater_from a f n')
+end. 
+
+(* It actually is just "repeat" from "prelims" in disguise *)
+Theorem repeater_from_repeat :
+forall a f n, repeater_from a f n = repeat f n a.
+Proof.
+intros a f n.
+induction n. { trivial. }
+simpl. rewrite IHn. trivial.
+Qed.
