new code/inv_ack.v
@@ -1,0 +1,25 @@
+Require Import Omega.
+Require Import prelims.
+Require Import countdown_repeater.
+Require Import inverse.
+Require Import countdown_compute.
+
+(*
+=============================================================================
+**************** SECTION 5: INVERSE OF KNUTH, ACKERMANN *********************
+=============================================================================
+*)
+
+(* ****** 5.1. HYPEROPS, KNUTH ARROWS, ACKERMANN ****************************)
+
+Fixpoint hyperop (n a b : nat) :=
+match n with
+| 0 => S b
+| S n1 => match n1 with
+          | 0 => repeater_from a (hyperop n1 a) b
+          | S n2 => match n2 with
+                    | 0 => repeater_from 0 (hyperop n2 a) b
+                    | S n3 => repeater_from 1 (hyperop n3 a) b
+                    end
+          end
+end.
