new code/inverse.v
@@ -1,0 +1,141 @@
+Require Import Omega.
+Require Import prelims.
+Require Import countdown_repeater.
+
+(*
+=============================================================================
+****************** SECTION 2: UPPER AND LOWER INVERSE RELATION **************
+=============================================================================
+*)
+
+(* This section is for upper (and lower, not yet complete) inverse relations
+   The upper inverse is much less painful to define and used in proofs
+   The lower inverse is hadrder because it does not always exists, thus
+   requires more attention to edge cases, which results in complicated proofs.
+   Also: (n - 2) is the upper inverse of (n + 2) but NOT the lower inverse *)
+
+(* ****** 2.1. UPPER AND LOWER INVERSES ***************** *)
+
+(* f is the upper inverse of F: f N is the smallest n such that F n >= N *)
+Definition upp_inv_rel (f F : nat -> nat) : Prop
+:= forall n N, f N <= n <-> N <= F n.
+
+(* f is the lower inverse of F: f N is the largest n such that F n <= N *)
+Definition low_inv_rel_from_a (a : nat) (f F : nat -> nat) : Prop
+:= forall n N, n <= f N <-> F n <= max a N.
+
+
+(* ****** 2.2. PROPERTIES PRESERVED BY INVERSES **************** *)
+
+(* Actually this section contains some redundant properties that I
+  haven't used in any proof *)
+
+(* Expansions, the counterpart of contractions *)
+Definition expanding (F : nat -> nat) : Prop
+:= forall n, n <= F n.
+
+Definition expand_strict_from (a : nat) (F : nat -> nat) : Prop
+:= forall n, (a <= n) -> (S n <= F n).
+
+(* If the upper inverse of "F" is a contraction, then "F" is an expansion *) 
+Lemma contract_upp_inv_expand :
+forall a f F, contract_strict_from (S a) f -> upp_inv_rel f F -> expand_strict_from a F.
+Proof.
+intros a f F Hf HfF n Han.
+rewrite <- (HfF n _).
+rewrite le_S_n_m.
+apply (Hf (S n)).
+rewrite <- le_S_n_m.
+apply Han.
+Qed.
+
+(* Basically, since "F" is an expansion, "F n >= 1 + n > 0" *)
+Lemma contract_upp_inv_positive :
+forall n f F, contract_strict_from 1 f -> upp_inv_rel f F -> (0 < F n).
+Proof.
+intros n f F Hf HfF.
+apply (Nat.le_trans _ (S n) _). { omega. }
+apply (contract_upp_inv_expand 0 f F); trivial.
+omega.
+Qed.
+
+(* If the upper inverse of "F" is increasing, so is "F" *)
+Lemma contract_incr_upp_inv_incr :
+forall f F, contract_strict_from 1 f -> increasing f -> upp_inv_rel f F -> increasing F.
+Proof.
+intros f F Hf_sh Hf_in HfF. rewrite incr_S. intro.
+rewrite <- (HfF (S n) _). apply (Nat.le_trans _ n _).
+- rewrite (HfF n _). trivial.
+- omega.
+Qed.
+
+(* Repeat preserves upper inverse relation *)
+Lemma upp_inv_repeat : forall k f F,
+upp_inv_rel f F -> upp_inv_rel (repeat f k) (repeat F k).
+Proof.
+unfold upp_inv_rel.
+intros k f F HfF.
+induction k.
+- intros n N. simpl. reflexivity.
+- intros n N. rewrite repeat_S_comm.
+  split.
+  + intro. rewrite IHk in H.
+    simpl. apply HfF. apply H.
+  + simpl. rewrite <- HfF.
+    rewrite IHk. trivial.
+Qed.
+
+(*
+Lemma contract_low_inv_positive :
+forall n f F, contract_strict_from 1 f -> low_inv_rel_from_a 1 f F
+-> (1 <= n) -> (0 < F n).
+Proof.
+intros n f F Hf HfF.
+apply (Nat.le_trans _ (S n) _). { omega. }
+apply (contract_low_inv_expand 1 f F); trivial.
+omega.
+Qed.
+
+Lemma contract_low_inv_expand :
+forall a f F, contract_strict_from a f -> low_inv_rel_from_a a f F -> expand_strict_from a F.
+Proof.
+intros a f F Hf HfF n Han.
+rewrite le_lt_S.
+rewrite <- not_le.
+assert (max a n = n) as Hman by (apply Nat.max_r_iff; trivial).
+rewrite <- Hman.
+rewrite <- (HfF _ n).
+rewrite Hman.
+apply (Hf n) in Han.
+omega.
+Qed.
+
+Lemma contract_incr_low_inv_incr :
+forall f F, contracting f -> increasing f -> low_inv_rel f F -> increasing F.
+Proof.
+intros f F Hf_sh Hf_in HfF. rewrite incr_S. intro.
+rewrite <- (HfF n _). apply (Nat.le_trans _ (S n) _).
+- omega.
+- rewrite (HfF (S n) _). trivial.
+Qed.
+*)
+
+(* ****** 2.3. COUNTDOWN - REPEATER - INVERSE PRESERVATION **************** *)
+
+(* This theorem is important. It says that the countdown and repeater will
+   preserve the upper inverse relation on their respective results
+   This is needed to prove that the tower (n - 2), ceil(n/2), ceil(log_2(n)), ...
+   is the upper inverse of the tower (n + 2), 2n, 2^n, ...
+   However I haven't cleaned that part in the old code yet *)
+
+Theorem countdown_repeater_upp_inverse : forall a f cf F,
+countdown_to_repeat_rel a f cf
+-> upp_inv_rel f F
+-> upp_inv_rel cf (repeater_from a F).
+Proof.
+intros a f cf F Hfcf HfF n N.
+rewrite repeater_from_repeat.
+rewrite (Hfcf N n).
+apply (upp_inv_repeat n _ _) in HfF.
+apply HfF.
+Qed.
